extraction: Clean up and split BinEncoders compiler

src/CertifiedExtraction/Benchmarks/BinEncoders.v
@@ -1,314 +1,59 @@
 Require Import CertifiedExtraction.Benchmarks.MicrobenchmarksSetup.
 Require Import BinEncoders.Env.Examples.Dns.
+Require Import BinEncodersProperties.
 
 Unset Implicit Arguments.
-
-Lemma push_function_into_destructuring_let2 {A1 A2 B C} :
-  forall (f: B -> C) (p: A1 * A2) (g : A1 -> A2 -> B),
-    f (match p with (a1, a2) => g a1 a2 end) =
-    match p with (a1, a2) => f (g a1 a2) end.
-Proof.
-  destruct p; reflexivity.
-Qed.
-
-Lemma push_function_into_destructuring_let3 {A1 A2 A3 B C} :
-  forall (f: B -> C) (p: A1 * A2 * A3) (g : A1 -> A2 -> A3 -> B),
-    f (match p with (a1, a2, a3) => g a1 a2 a3 end) =
-    match p with (a1, a2, a3) => f (g a1 a2 a3) end.
-Proof.
-  repeat destruct p; reflexivity.
-Qed.
-
-Lemma CompileDestructuringLet2 {A1 A2 B av: Type} :
-  forall tenv1 tenv2 (k: NameTag av B) k1 k2 (pair: A1 * A2) ext env (g: A1 -> A2 -> Comp B) prog cleanup,
-    {{ tenv1 }}
-      prog
-    {{ [[k1 <-- fst pair as a1]]::[[k2 <-- snd pair as a2]]::[[k <~~ g a1 a2 as v]] :: tenv2 v }} ∪ {{ ext }} // env ->
-    {{ [[k1 <-- fst pair as a1]]::[[k2 <-- snd pair as a2]]::[[k <~~ g a1 a2 as v]] :: tenv2 v }}
-      cleanup
-    {{ [[k <~~ g (fst pair) (snd pair) as v]] :: tenv2 v }} ∪ {{ ext }} // env ->
-    {{ tenv1 }}
-      Seq prog cleanup
-    {{ [[k <~~ let (a1, a2) := pair in g a1 a2 as v]] :: tenv2 v }} ∪ {{ ext }} // env.
-Proof.
-  destruct pair; simpl; SameValues_Facade_t.
-Qed.
-
-Lemma CompileDestructuringLet2_ret {A1 A2 B av: Type} :
-  forall tenv1 tenv2 (k: NameTag av B) k1 k2 (pair: A1 * A2) ext env (g: A1 -> A2 -> B) prog cleanup,
-    {{ tenv1 }}
-      prog
-    {{ [[k1 <-- fst pair as a1]]::[[k2 <-- snd pair as a2]]::[[k <-- g a1 a2 as v]] :: tenv2 v }} ∪ {{ ext }} // env ->
-    {{ [[k1 <-- fst pair as a1]]::[[k2 <-- snd pair as a2]]::[[k <-- g a1 a2 as v]] :: tenv2 v }}
-      cleanup
-    {{ [[k <-- g (fst pair) (snd pair) as v]] :: tenv2 v }} ∪ {{ ext }} // env ->
-    {{ tenv1 }}
-      Seq prog cleanup
-    {{ [[k <-- let (a1, a2) := pair in g a1 a2 as v]] :: tenv2 v }} ∪ {{ ext }} // env.
-Proof.
-  destruct pair; simpl; SameValues_Facade_t.
-Qed.
-
-Lemma CompileDestructuringLet23_ret {A11 A12 A2 B av: Type} :
-  forall tenv1 tenv2 (k: NameTag av B) k11 k12 k2 (pair: A11 * A12 * A2) ext env (g: A11 * A12 -> A2 -> B) prog cleanup,
-    {{ tenv1 }}
-      prog
-    {{ [[k11 <-- fst (fst pair) as a11]]
-         ::[[k12 <-- snd (fst pair) as a12]]
-         ::[[k2 <-- snd pair as a2]]
-         ::[[k <-- g (a11, a12) a2 as v]]
-         :: tenv2 v }} ∪ {{ ext }} // env ->
-    {{ [[k11 <-- fst (fst pair) as a11]]
-         ::[[k12 <-- snd (fst pair) as a12]]
-         ::[[k2 <-- snd pair as a2]]
-         ::[[k <-- g (a11, a12) a2 as v]]
-         :: tenv2 v }}
-      cleanup
-    {{ [[k <-- g (fst pair) (snd pair) as v]] :: tenv2 v }} ∪ {{ ext }} // env ->
-    {{ tenv1 }}
-      Seq prog cleanup
-    {{ [[k <-- let (a1, a2) := pair in g a1 a2 as v]] :: tenv2 v }} ∪ {{ ext }} // env.
-Proof.
-  destruct pair; simpl; SameValues_Facade_t.
-Qed.
-
-Lemma CompileDestructuringLet23'_ret {A11 A12 A2 B av: Type} :
-  forall tenv1 tenv2 (k: NameTag av B) k12 k2 (pair: A11 * A12 * A2) ext env (g: A11 * A12 -> A2 -> B) prog cleanup,
-    {{ tenv1 }}
-      prog
-    {{ [[k12 <-- snd (fst pair) as a12]]
-         ::[[k2 <-- snd pair as a2]]
-         ::[[k <-- g (fst (fst pair), a12) a2 as v]]
-         :: tenv2 v }} ∪ {{ ext }} // env ->
-    {{ [[k12 <-- snd (fst pair) as a12]]
-         ::[[k2 <-- snd pair as a2]]
-         ::[[k <-- g (fst (fst pair), a12) a2 as v]]
-         :: tenv2 v }}
-      cleanup
-    {{ [[k <-- g (fst pair) (snd pair) as v]] :: tenv2 v }} ∪ {{ ext }} // env ->
-    {{ tenv1 }}
-      Seq prog cleanup
-    {{ [[k <-- let (a1, a2) := pair in g a1 a2 as v]] :: tenv2 v }} ∪ {{ ext }} // env.
-Proof.
-  destruct pair; simpl; SameValues_Facade_t.
-Qed.
-
-(* Remove Printing Let prod. *)
 
 Require Import CertifiedExtraction.Extraction.QueryStructures.CallRules.Core.
 Require Import CertifiedExtraction.Extraction.External.Loops.
 Require Import CertifiedExtraction.Extraction.External.FacadeLoops.
-Require Import CallRules.TupleList.
 
 Check miniChomp.
+(* FIXME Rename SameValues_remove_SCA to SameValues_remove_W *)
 
-Lemma miniChomp_0:
-  forall {A av} (k k': NameTag av _) (v: Comp A) tenv tenv' ext prog env,
-    (forall vv: A, v ↝ vv ->
-           {{ [[k  <--  vv as vv]] :: tenv vv }} prog {{ [[k' <--  vv as vv]] :: tenv' vv }} ∪ {{ ext }} // env) ->
-    {{ [[k <~~ v as vv]] :: (tenv vv) }} prog {{ [[k' <~~ v as vv]] :: tenv' vv }} ∪ {{ ext }} // env.
-Proof.
-  miniChomp_t; destruct k, k'; simpl; miniChomp_t;
+Ltac decide_NotInTelescope ::=  (* FIXME merge *)
+  progress repeat match goal with
+                  | _ => cleanup
+                  | _ => congruence
+                  | [  |- NotInTelescope _ Nil ] => reflexivity
+                  | [  |- NotInTelescope ?k (Cons _ _ _) ] => simpl
+                  | _ => auto 1  (* Added for tricky cases like CompileLoopBase2 *)
+                  end.
+
+Ltac compile_simple_inplace ::=
+  match_ProgOk                (* FIXME merge this upstream (made it faster in the failing case) *)
+  ltac:(fun prog pre post ext env =>
+          match post with
+          | Cons (NTSome ?s) (ret (?op ?a' ?b)) ?tenv' =>
+            match pre with
+            | context[Cons (NTSome ?s) (ret ?a) _] =>
+              unify a a';
+              is_word (op a b);
+              let facade_op := translate_op op in
+              move_to_front s;
+              first [ apply (CompileBinopOrTest_right_inPlace_tel facade_op)
+                    | apply (CompileBinopOrTest_right_inPlace_tel_generalized facade_op) ]
+            end
+          end).
+
+Ltac decide_TelEq_instantiate_step ::= (* FIXME merge  *)
   match goal with
-  | [ H: context[NTNone] |- _ ] => rewrite Propagate_anonymous_ret in H
-  end; miniChomp_t.
-Qed.
+  | [  |- TelEq _ ?from ?to ] =>
+    match constr:((from, to)) with
+    | _ => rewrite DropName_Cons_Some_eq by congruence
+    | _ => rewrite DropName_Cons_Some_neq by congruence
+    | _ => (is_evar from || is_evar to); apply TelEq_refl
+    | (Cons NTNone _ _, _) => apply TelEq_chomp_None_left; [ eexists; reflexivity | red; intros ]
+    | (_, Cons NTNone _ _) => apply TelEq_chomp_None_right; [ eexists; reflexivity | red; intros ]
+    | (Cons ?k _ _, ?t) => decide_TelEq_instantiate_do_swaps k t; apply TelEq_chomp_head; red; intros
+    | (?t, Cons ?k _ _) => decide_TelEq_instantiate_do_swaps k t; apply TelEq_chomp_head; red; intros
+    | context [DropName ?k ?tenv] => first [ is_dirty_telescope tenv; fail 1 |
+                                            rewrite (DropName_NotInTelescope tenv k) by eauto ]
+    | _ => apply TelEq_refl
+    end
+  end.
 
-Lemma CompileLoopBase2 :
-  forall {A1 A2 C}
-    `{FacadeWrapper (Value QsADTs.ADTValue) A1}
-    `{FacadeWrapper (Value QsADTs.ADTValue) A2}
-    `{FacadeWrapper (Value QsADTs.ADTValue) C}
-    `{FacadeWrapper (Value QsADTs.ADTValue) (list C)}
-    (lst: list C) init vhead vtest vlst vret1 vret2
-    fpop fempty fdealloc facadeBody env (ext: StringMap.t (Value QsADTs.ADTValue)) tenv
-    (f: A1 * A2 -> C -> A1 * A2),
-    (* GLabelMap.MapsTo fpop (Axiomatic QsADTs.TupleList_pop) env -> *)
-    (* GLabelMap.MapsTo fempty (Axiomatic QsADTs.TupleList_empty) env -> *)
-    (* GLabelMap.MapsTo fdealloc (Axiomatic QsADTs.TupleList_delete) env -> *)
-    PreconditionSet tenv ext [[[vhead; vtest; vlst; vret1; vret2]]] ->
-    (forall head (acc1: A1) (acc2: A2) (s: list C),
-        {{ [[`vret1 <-- acc1 as _]] :: [[`vret2 <-- acc2 as _]] :: [[`vhead <-- head as _]] :: tenv }}
-          facadeBody
-        {{ [[`vret1 <-- fst (f (acc1, acc2) head) as _]] :: [[`vret2 <-- snd (f (acc1, acc2) head) as _]] :: tenv }} ∪
-        {{ [vtest <-- wrap (bool2w false)] :: [vlst <-- wrap s] :: ext }} // env) ->
-    {{ [[`vret1 <-- fst init as _]] :: [[`vret2 <-- snd init as _]] :: [[`vlst <-- lst as _]] :: tenv }}
-      (Seq (Fold vhead vtest vlst fpop fempty facadeBody) (Call (DummyArgument vtest) fdealloc (vlst :: nil)))
-    {{ [[`vret1 <-- fst (fold_left f lst init) as _]] :: [[`vret2 <-- snd (fold_left f lst init) as _]] :: tenv }} ∪ {{ ext }} // env.
-Proof.
-  Transparent DummyArgument.
-  unfold DummyArgument; loop_t.
-
-  move_to_front vlst.
-  instantiate (1 := [[`vlst <-- lst as ls]] :: [[`vtest <-- (bool2w match ls with
-                                                              | nil => true
-                                                              | _ :: _ => false
-                                                              end) as _]] :: [[ ` vret1 <-- fst init as _]]::[[ ` vret2 <-- snd init as _]]::tenv); admit.
-  (* eapply (CompileTupleList_Empty_alt (N := N)); loop_t. *)
-
-  2:instantiate (1 := [[ ` vlst <-- nil as _]]::[[ ` vret1 <-- fst (fold_left f lst init) as _]]::[[ ` vret2 <-- snd (fold_left f lst init) as _]]::tenv); admit.
-
-  loop_t.
-  generalize dependent init;
-  induction lst; loop_t.
-
-  move_to_front vtest;
-    apply CompileWhileFalse_Loop; loop_t.
-  simpl.
-
-  eapply CompileWhileTrue; [ loop_t.. | ].
-
-  instantiate (1 := [[ `vhead <-- a as _ ]] :: [[ `vlst <-- lst as _ ]] :: [[ ` vtest <-- W0 as _]]::[[ ` vret1 <-- fst init as _]]::[[ ` vret2 <-- snd init as _]]::tenv); admit.
-
-  (* rewrite <- GLabelMapFacts.find_mapsto_iff; assumption. *)
-
-  move_to_front vlst; apply ProgOk_Chomp_Some; loop_t.
-  move_to_front vtest; apply ProgOk_Chomp_Some; loop_t.
-  move_to_front vret2; loop_t.
-  move_to_front vret1; loop_t.
-  computes_to_inv; subst; defunctionalize_evar; eauto.
-
-  move_to_front vtest.
-  apply ProgOk_Remove_Skip_L; hoare.
-  apply CompileDeallocSCA_discretely; try compile_do_side_conditions.
-  apply ProgOk_Chomp_Some; try compile_do_side_conditions; intros.
-  apply CompileSkip.
-
-  instantiate (1 := [[ ` vlst <-- lst as ls]]
-                     :: [[`vtest <-- (bool2w match ls with
-                                          | nil => true
-                                          | _ :: _ => false
-                                          end) as _]]
-                     ::[[ ` vret1 <-- fst (f (fst init, snd init) a) as _]]
-                     ::[[ ` vret2 <-- snd (f (fst init, snd init) a) as _]]::tenv); admit.
-  (* apply CompileTupleList_Empty_alt; loop_t. *)
-
-  rewrite <- surjective_pairing.
-  loop_t.
-Qed.
-
-Lemma CompileLoop2 :
-  forall {A1 A2 C}
-    `{FacadeWrapper (Value QsADTs.ADTValue) A1}
-    `{FacadeWrapper (Value QsADTs.ADTValue) A2}
-    `{FacadeWrapper (Value QsADTs.ADTValue) C}
-    `{FacadeWrapper (Value QsADTs.ADTValue) (list C)}
-    (lst: list C) init vhead vtest vlst vret1 vret2
-    fpop fempty fdealloc facadeBody facadeConclude
-    env (ext: StringMap.t (Value QsADTs.ADTValue)) tenv tenv'
-    (f: A1 * A2 -> C -> A1 * A2),
-    (* GLabelMap.MapsTo fpop (Axiomatic (QsADTs.TupleList_pop)) env -> *)
-    (* GLabelMap.MapsTo fempty (Axiomatic (QsADTs.TupleList_empty)) env -> *)
-    (* GLabelMap.MapsTo fdealloc (Axiomatic (QsADTs.TupleList_delete)) env -> *)
-    PreconditionSet tenv ext [[[vhead; vtest; vlst; vret1; vret2]]] ->
-    {{ [[`vret1 <-- fst (fold_left f lst init) as _]] :: [[`vret2 <-- snd (fold_left f lst init) as _]] :: tenv }}
-      facadeConclude
-    {{ [[`vret1 <-- fst (fold_left f lst init) as v1]] :: [[`vret2 <-- snd (fold_left f lst init) as v2]] :: tenv' v1 v2}} ∪ {{ ext }} // env ->
-    (forall head (acc1: A1) (acc2: A2) (s: list C),
-        {{ [[`vret1 <-- acc1 as _]] :: [[`vret2 <-- acc2 as _]] :: [[`vhead <-- head as _]] :: tenv }}
-          facadeBody
-        {{ [[`vret1 <-- fst (f (acc1, acc2) head) as _]] :: [[`vret2 <-- snd (f (acc1, acc2) head) as _]] :: tenv }} ∪
-        {{ [vtest <-- wrap (bool2w false)] :: [vlst <-- wrap s] :: ext }} // env) ->
-    {{ [[`vret1 <-- fst init as _]] :: [[`vret2 <-- snd init as _]] :: [[`vlst <-- lst as _]] :: tenv }}
-      (Seq (Seq (Fold vhead vtest vlst fpop fempty facadeBody) (Call (DummyArgument vtest) fdealloc (vlst :: nil))) facadeConclude)
-    {{ [[`vret1 <-- fst (fold_left f lst init) as v1]] :: [[`vret2 <-- snd (fold_left f lst init) as v2]] :: tenv' v1 v2 }} ∪ {{ ext }} // env.
-Proof.
-  hoare. hoare.
-  eapply @CompileLoopBase2; eassumption.
-Qed.
-
-Lemma CompileLoop2_Alloc :
-  forall {A1 A2 C}
-    `{FacadeWrapper (Value QsADTs.ADTValue) A1}
-    `{FacadeWrapper (Value QsADTs.ADTValue) A2}
-    `{FacadeWrapper (Value QsADTs.ADTValue) C}
-    `{FacadeWrapper (Value QsADTs.ADTValue) (list C)}
-    vhead vtest (lst: list C) init vlst vret1 vret2
-    env (ext: StringMap.t (Value QsADTs.ADTValue)) tenv tenv'
-    (f: A1 * A2 -> C -> A1 * A2)
-    fpop fempty fdealloc facadeInit facadeBody facadeConclude,
-    (* GLabelMap.MapsTo fpop (Axiomatic (QsADTs.TupleList_pop)) env -> *)
-    (* GLabelMap.MapsTo fempty (Axiomatic (QsADTs.TupleList_empty)) env -> *)
-    (* GLabelMap.MapsTo fdealloc (Axiomatic (QsADTs.TupleList_delete)) env -> *)
-    PreconditionSet tenv ext [[[vhead; vtest; vlst; vret1; vret2]]] ->
-    {{ [[`vlst <-- lst as _]] :: tenv }}
-      facadeInit
-    {{ [[`vret1 <-- fst init as _]] :: [[`vret2 <-- snd init as _]] :: [[`vlst <-- lst as _]] :: tenv }} ∪ {{ ext }} // env ->
-    {{ [[`vret1 <-- fst (fold_left f lst init) as _]] :: [[`vret2 <-- snd (fold_left f lst init) as _]] :: tenv }}
-      facadeConclude
-    {{ [[`vret1 <-- fst (fold_left f lst init) as v1]] :: [[`vret2 <-- snd (fold_left f lst init) as v2]] :: tenv' v1 v2 }} ∪ {{ ext }} // env ->
-    (forall head (acc1: A1) (acc2: A2) (s: list C),
-        {{ [[`vret1 <-- acc1 as _]] :: [[`vret2 <-- acc2 as _]] :: [[`vhead <-- head as _]] :: tenv }}
-          facadeBody
-        {{ [[`vret1 <-- fst (f (acc1, acc2) head) as _]] :: [[`vret2 <-- snd (f (acc1, acc2) head) as _]] :: tenv }} ∪
-        {{ [vtest <-- wrap (bool2w false)] :: [vlst <-- wrap s] :: ext }} // env) ->
-    {{ [[`vlst <-- lst as _]] :: tenv }}
-      (Seq facadeInit (Seq (Seq (Fold vhead vtest vlst fpop fempty facadeBody) (Call (DummyArgument vtest) fdealloc (vlst :: nil))) facadeConclude))
-    {{ [[`vret1 <-- fst (fold_left f lst init) as v1]] :: [[`vret2 <-- snd (fold_left f lst init) as v2]] :: tenv' v1 v2 }} ∪ {{ ext }} // env.
-Proof.
-  hoare. hoare.
-  eapply @CompileLoop2; try eassumption.
-Qed.
-
-Lemma CompileAppendBool :
-  forall {av} {W: FacadeWrapper av (list bool)} vout vbools vbool
-    (tenv: Telescope av) tenv' ext env fappend facadeConclude bools b,
-    {{ [[ ` vbools <-- bools ++ b :: nil as _]] :: [[ ` vbool <-- b as _]] :: tenv }}
-      facadeConclude
-    {{ [[ ` vbools <-- bools ++ b :: nil as vbls]] :: tenv' vbls }} ∪ {{ ext }} // env ->
-    {{ [[ ` vbools <-- bools as _]] :: [[ ` vbool <-- b as _]] :: tenv }}
-      Seq (Call (DummyArgument vout) fappend (vbools :: nil)) facadeConclude
-    {{ [[ ` vbools <-- bools ++ b :: nil as bls]] :: tenv' bls }} ∪ {{ ext }} // env.
-Proof.
-  repeat hoare.
-  admit.
-Qed.
-
-Lemma CompileExtendLifetime':
-  forall {av A} {env ext} (k: NameTag av A) comp tenv tenv' prog dealloc,
-    {{ [[k <~~ comp as kk]] :: tenv kk }}
-      prog
-    {{ [[k <~~ comp as _]] :: tenv' }} ∪ {{ext}} // env ->
-    {{ [[k <~~ comp as _]] :: tenv' }}
-      dealloc
-    {{ [[comp as _]] :: tenv' }} ∪ {{ext}} // env ->
-    {{ [[k <~~ comp as kk]] :: tenv kk }}
-      (Seq prog dealloc)
-    {{ tenv' }} ∪ {{ext}} // env.
-Proof.
-  SameValues_Facade_t.
-Qed.
-
-(* (* This code gets the TC resolution in a loop *)
-
-Instance FacadeWrapper_bool : FacadeWrapper W bool.
-Proof.
-  refine {| wrap v := (bool2w v) |};
-    abstract (intros * H; inversion H; eauto using bool2w_inj).
-Defined.
-
-Instance FacadeWrapper_trans {A B C} :
-  FacadeWrapper C B ->
-  FacadeWrapper B A ->
-  FacadeWrapper C A.
-Proof.
-  intros; refine {| wrap := fun (a : A) => wrap (wrap a: B): C |}.
-  intros; do 2 apply wrap_inj; assumption.
-Qed.
-
-(* Typeclasses eauto := debug dfs. *)
-
-Lemma CompileDeallocSCA_discretely :
-  forall {av} {A} (H: FacadeWrapper W A) (tenv tenv': Telescope av) ext env k (v: Comp A) prog,
-    k ∉ ext ->
-    NotInTelescope k tenv ->
-    {{ [[`k <~~ v as _]] :: tenv }} prog {{ [[`k <~~ v as _]] :: tenv' }} ∪ {{ ext }} // env ->
-    {{ [[`k <~~ v as _]] :: tenv }} prog {{ tenv' }} ∪ {{ ext }} // env.
-Proof.
-  SameValues_Facade_t.
-Qed. *)
-
-(* Rename SameValues_remove_SCA to SameValues_remove_W *)
+(* FIXME merge thee general lemmas about non-adts, renaming the existing versions to _W *)
 
 Lemma SameValues_remove_SCA:
   forall (av : Type) {A} (Wrapper: FacadeWrapper (Value av) A),
@@ -414,146 +159,30 @@ Proof.
   SameValues_Facade_t.
 Qed.
 
-Definition encode_continue {E B}
-           (transformer : Transformer.Transformer B)
-           (encode : E -> B * E)
-           acc :=
-  let (p, e') := encode (snd acc) in
-  (Transformer.transform (fst acc) p, e').
-
-Definition compose_acc {E B}
-           (transformer : Transformer.Transformer B)
-           (encode1 : E -> B * E)
-           (encode2 : E -> B * E) e0 :=
-  encode_continue transformer encode2 (encode1 e0).
-
-Lemma Compose_compose_acc {E B} :
-  forall transformer encode1 encode2 e0,
-    @Compose.compose E B transformer encode1 encode2 e0 =
-    @compose_acc E B transformer encode1 encode2 e0.
-Proof.
-  intros; unfold compose_acc, Compose.compose, encode_continue.
-  destruct (encode1 _); simpl; destruct (encode2 _); reflexivity.
-Qed.
-
 Lemma CompileCompose :
-  forall {av} E B (transformer: Transformer.Transformer B) enc1 enc2 (vstream: NameTag av B) (vcache: NameTag av E) (cstream_cache: B * E) tenv ext env p1 p2,
-    {{ [[ NTNone  <--  cstream_cache as stream_cache ]]
-         :: [[ vstream  <--  (fst stream_cache) as stream ]]
-         :: [[ vcache  <--  (snd stream_cache) as cache ]]
-         :: tenv }}
-      p1
-    {{ [[ NTNone  <--  cstream_cache as stream_cache ]]
-         :: [[ NTNone  <--  enc1 (snd cstream_cache) as encoded1 ]]
-         :: [[ vstream  <--  Transformer.transform (fst stream_cache) (fst encoded1) as stream1 ]]
-         :: [[ vcache  <--  (snd encoded1) as cache1 ]]
-         :: tenv }} ∪ {{ ext }} // env ->
-    {{ [[ NTNone  <--  cstream_cache as stream_cache ]]
-         :: [[ NTNone  <--  enc1 (snd cstream_cache) as encoded1 ]]
-         :: [[ vstream  <--  Transformer.transform (fst stream_cache) (fst encoded1) as stream1 ]]
-         :: [[ vcache  <--  (snd encoded1) as cache1 ]]
-         :: tenv }}
-      p2
-    {{ [[ NTNone  <--  cstream_cache as stream_cache ]]
-         :: [[ NTNone  <--  enc1 (snd cstream_cache) as encoded1 ]]
-         :: [[ NTNone  <--  enc2 (snd encoded1) as encoded2 ]]
-         :: [[ vstream  <--  Transformer.transform (Transformer.transform (fst stream_cache) (fst encoded1)) (fst encoded2) as stream2 ]]
-         :: [[ vcache  <--  (snd encoded2) as cache2 ]]
-         :: tenv }} ∪ {{ ext }} // env ->
-    {{ [[ NTNone  <--  cstream_cache as stream_cache ]]
-         :: [[ vstream  <--  (fst stream_cache) as stream ]]
-         :: [[ vcache  <--  (snd stream_cache) as cache ]]
-         :: tenv }}
-      (Seq p1 p2)
-    {{ [[ NTNone  <--  cstream_cache as stream_cache ]]
-         :: [[ NTNone  <--  @Compose.compose E B transformer enc1 enc2 (snd stream_cache) as composed ]]
-         :: [[ vstream  <--  Transformer.transform (fst stream_cache) (fst composed) as stream ]]
-         :: [[ vcache  <--  (snd composed) as cache ]]
-         :: tenv }} ∪ {{ ext }} // env.
-Proof.
-  repeat hoare.
-  setoid_rewrite Compose_compose_acc.
-  unfold compose_acc, encode_continue.
-  repeat setoid_rewrite Propagate_anonymous_ret.
-  repeat setoid_rewrite Propagate_anonymous_ret in H.
-  repeat setoid_rewrite Propagate_anonymous_ret in H0.
-  destruct cstream_cache; simpl in *.
-  destruct (enc1 _); simpl in *.
-  destruct (enc2 _); simpl in *.
-  rewrite Transformer.transform_assoc; assumption.
-Qed.
-
-Lemma CompileCompose_spec :
-  forall {av} E B (transformer: Transformer.Transformer B) enc1 enc2 (vstream: NameTag av B) (vcache: NameTag av E) (stream_cache: B * E) tenv ext env p1 p2,
-    {{ [[ vstream  <--  (fst stream_cache) as stream ]]
-         :: [[ vcache  <--  (snd stream_cache) as cache ]]
-         :: tenv }}
-      p1
-    {{ [[ NTNone  <--  enc1 (snd stream_cache) as encoded1 ]]
-         :: [[ vstream  <--  Transformer.transform (fst stream_cache) (fst encoded1) as stream1 ]]
-         :: [[ vcache  <--  (snd encoded1) as cache1 ]]
-         :: tenv }} ∪ {{ ext }} // env ->
-    {{ [[ NTNone  <--  enc1 (snd stream_cache) as encoded1 ]]
-         :: [[ vstream  <--  Transformer.transform (fst stream_cache) (fst encoded1) as stream1 ]]
-         :: [[ vcache  <--  (snd encoded1) as cache1 ]]
-         :: tenv }}
-      p2
-    {{ [[ NTNone  <--  enc1 (snd stream_cache) as encoded1 ]]
-         :: [[ NTNone  <--  enc2 (snd encoded1) as encoded2 ]]
-         :: [[ vstream  <--  Transformer.transform (Transformer.transform (fst stream_cache) (fst encoded1)) (fst encoded2) as stream2 ]]
-         :: [[ vcache  <--  (snd encoded2) as cache2 ]]
-         :: tenv }} ∪ {{ ext }} // env ->
-    {{ [[ vstream  <--  (fst stream_cache) as stream ]]
-         :: [[ vcache  <--  (snd stream_cache) as cache ]]
-         :: tenv }}
-      (Seq p1 p2)
-    {{ [[ NTNone  <--  @Compose.compose E B transformer enc1 enc2 (snd stream_cache) as composed ]]
-         :: [[ vstream  <--  Transformer.transform (fst stream_cache) (fst composed) as stream ]]
-         :: [[ vcache  <--  (snd composed) as cache ]]
-         :: tenv }} ∪ {{ ext }} // env.
-Proof.
-  repeat hoare.
-  setoid_rewrite Compose_compose_acc.
-  unfold compose_acc, encode_continue.
-  repeat setoid_rewrite Propagate_anonymous_ret.
-  repeat setoid_rewrite Propagate_anonymous_ret in H.
-  repeat setoid_rewrite Propagate_anonymous_ret in H0.
-  destruct stream_cache; simpl in *.
-  destruct (enc1 _); simpl in *.
-  destruct (enc2 _); simpl in *.
-  rewrite Transformer.transform_assoc; assumption.
-Qed.
-
-Lemma CompileCompose_spec' :
   forall {av} E B (transformer: Transformer.Transformer B) enc1 enc2
-    (vstream: NameTag av B) (vcache: NameTag av E) (stream: B) (cache: E)
-    tenv tenv' tenv'' ext env p1 p2,
+    (vstream: NameTag av B) (stream: B) (cache: E)
+    cacheF (tenv tenv' tenv'': Telescope av) ext env p1 p2,
     {{ [[ vstream  <--  stream as _ ]]
-         :: [[ vcache  <--  cache as _ ]]
-         :: tenv }}
+         :: cacheF tenv cache }}
       p1
     {{ [[ NTNone  <--  enc1 cache as encoded1 ]]
          :: [[ vstream  <--  Transformer.transform stream (fst encoded1) as stream1 ]]
-         :: [[ vcache  <--  (snd encoded1) as cache1 ]]
-         :: tenv' }} ∪ {{ ext }} // env ->
+         :: cacheF tenv' (snd encoded1) }} ∪ {{ ext }} // env ->
     (let encoded1 := enc1 cache in
      let stream1 := Transformer.transform stream (fst encoded1) in
      {{ [[ vstream  <--  stream1 as _ ]]
-         :: [[ vcache  <--  (snd encoded1) as cache1 ]]
-          :: tenv' }}
+          :: cacheF tenv' (snd encoded1) }}
        p2
      {{ [[ NTNone  <--  enc2 (snd encoded1) as encoded2 ]]
           :: [[ vstream  <--  Transformer.transform stream1 (fst encoded2) as stream2 ]]
-          :: [[ vcache  <--  (snd encoded2) as cache2 ]]
-          :: tenv'' }} ∪ {{ ext }} // env) ->
+          :: cacheF tenv'' (snd encoded2) }} ∪ {{ ext }} // env) ->
     {{ [[ vstream  <--  stream as _ ]]
-         :: [[ vcache  <--  cache as _ ]]
-         :: tenv }}
+         :: cacheF tenv cache }}
       (Seq p1 p2)
     {{ [[ NTNone  <--  @Compose.compose E B transformer enc1 enc2 cache as composed ]]
          :: [[ vstream  <--  Transformer.transform stream (fst composed) as stream ]]
-         :: [[ vcache  <--  (snd composed) as cache ]]
-         :: tenv'' }} ∪ {{ ext }} // env.
+         :: cacheF tenv'' (snd composed) }} ∪ {{ ext }} // env.
 Proof.
   repeat hoare.
   setoid_rewrite Compose_compose_acc.
@@ -567,28 +196,35 @@ Proof.
   rewrite Transformer.transform_assoc; assumption.
 Qed.
 
-Lemma ProgOk_Add_snd :
-  forall {A B av} (kfst: NameTag av _) (ksnd: NameTag av _) (cpair: Comp (A * B)) tenv tenv' ext env p1 p2,
-    {{ tenv }}
+Lemma CompileCompose_init :
+  forall {av} E B (transformer: Transformer.Transformer B) enc1 enc2
+    (vstream: NameTag av B) (cache: E)
+    cacheF (tenv tenv' tenv'': Telescope av) ext env p1 p2,
+    {{ [[ vstream  <--  Transformer.transform_id as _ ]]
+         :: cacheF tenv cache }}
       p1
-    {{ [[ NTNone  <~~  cpair as pair ]]
-         :: [[ kfst  <--  fst pair as p1 ]]
-         :: [[ ksnd  <--  snd pair as p2 ]]
-         :: tenv' pair }} ∪ {{ ext }} // env ->
-    {{ [[ NTNone  <~~  cpair as pair ]]
-         :: [[ kfst  <--  fst pair as p1 ]]
-         :: [[ ksnd  <--  snd pair as p2 ]]
-         :: tenv' pair }}
-      p2
-    {{ [[ NTNone  <~~  cpair as pair ]]
-         :: [[ kfst  <--  fst pair as p1 ]]
-         :: tenv' pair }} ∪ {{ ext }} // env ->
-    {{ tenv }}
+    {{ [[ NTNone  <--  enc1 cache as encoded1 ]]
+         :: [[ vstream  <--  Transformer.transform Transformer.transform_id (fst encoded1) as stream1 ]]
+         :: cacheF tenv' (snd encoded1) }} ∪ {{ ext }} // env ->
+    (let encoded1 := enc1 cache in
+     {{ [[ vstream  <--  (fst encoded1) as _ ]]
+          :: cacheF tenv' (snd encoded1) }}
+       p2
+     {{ [[ NTNone  <--  enc2 (snd encoded1) as encoded2 ]]
+          :: [[ vstream  <--  Transformer.transform (fst encoded1) (fst encoded2) as stream2 ]]
+          :: cacheF tenv'' (snd encoded2) }} ∪ {{ ext }} // env) ->
+    {{ [[ vstream  <--  Transformer.transform_id as _ ]]
+         :: cacheF tenv cache }}
       (Seq p1 p2)
-    {{ [[ NTNone  <~~  cpair as pair ]]
-         :: [[ kfst  <--  fst pair as p1 ]] :: tenv' pair }} ∪ {{ ext }} // env.
+    {{ [[ NTNone  <--  @Compose.compose E B transformer enc1 enc2 cache as composed ]]
+         :: [[ vstream  <--  (fst composed) as stream ]]
+         :: cacheF tenv'' (snd composed) }} ∪ {{ ext }} // env.
 Proof.
-  repeat hoare.
+  intros.
+  setoid_rewrite <- (Transformer.transform_id_left (fst _)).
+  eapply CompileCompose; cbv zeta.
+  eassumption.
+  setoid_rewrite Transformer.transform_id_left; eassumption.
 Qed.
 
 Lemma ProgOk_Add_snd_ret :
@@ -616,12 +252,6 @@ Proof.
   assumption.
 Qed.
 
-Ltac compile_compose_internal :=
-  eapply CompileCompose_spec';
-  [ | intros;
-      let stream := fresh "stream" in
-      set (Transformer.transform _ _) as stream ].
-
 Definition PacketAsCollectionOfVariables
            {av} vid vmask vquestion vanswer vauthority vadditional tail (p: packet_t)
   : Telescope av :=
@@ -641,90 +271,22 @@ Definition DnsCacheAsCollectionOfVariables
     :: [[ voffs <-- c.(DnsMap.offs) as _ ]]
     :: tail.
 
-Lemma CompileLoop2_destructed :
-  forall {A1 A2 C}
-    `{FacadeWrapper (Value QsADTs.ADTValue) A1}
-    `{FacadeWrapper (Value QsADTs.ADTValue) A2}
-    `{FacadeWrapper (Value QsADTs.ADTValue) C}
-    `{FacadeWrapper (Value QsADTs.ADTValue) (list C)}
-    vhead vtest vlst vret1 vret2
-    (lst: list C) init1 init2 (init := (init1, init2))
-    fpop fempty fdealloc facadeBody facadeConclude
-    env (ext: StringMap.t (Value QsADTs.ADTValue)) tenv tenv'
-    (f: A1 * A2 -> C -> A1 * A2),
-    (* GLabelMap.MapsTo fpop (Axiomatic (QsADTs.TupleList_pop)) env -> *)
-    (* GLabelMap.MapsTo fempty (Axiomatic (QsADTs.TupleList_empty)) env -> *)
-    (* GLabelMap.MapsTo fdealloc (Axiomatic (QsADTs.TupleList_delete)) env -> *)
-    PreconditionSet tenv ext [[[vhead; vtest; vlst; vret1; vret2]]] ->
-    {{ [[`vret1 <-- fst (fold_left f lst init) as _]] :: [[`vret2 <-- snd (fold_left f lst init) as _]] :: tenv }}
-      facadeConclude
-    {{ [[`vret1 <-- fst (fold_left f lst init) as v1]] :: [[`vret2 <-- snd (fold_left f lst init) as v2]] :: tenv' v1 v2}} ∪ {{ ext }} // env ->
-    (forall head (acc1: A1) (acc2: A2) (s: list C),
-        {{ [[`vret1 <-- acc1 as _]] :: [[`vret2 <-- acc2 as _]] :: [[`vhead <-- head as _]] :: tenv }}
-          facadeBody
-        {{ [[`vret1 <-- fst (f (acc1, acc2) head) as _]] :: [[`vret2 <-- snd (f (acc1, acc2) head) as _]] :: tenv }} ∪
-        {{ [vtest <-- wrap (bool2w false)] :: [vlst <-- wrap s] :: ext }} // env) ->
-    {{ [[`vlst <-- lst as _]] :: [[`vret1 <-- init1 as _]] :: [[`vret2 <-- init2 as _]] :: tenv }}
-      (Seq (Seq (Fold vhead vtest vlst fpop fempty facadeBody) (Call (DummyArgument vtest) fdealloc (vlst :: nil))) facadeConclude)
-    {{ [[ ret (fold_left f lst init) as folded ]]
-         :: [[`vret1 <-- fst folded as v1]]
-         :: [[`vret2 <-- snd folded as v2]]
-         :: tenv' v1 v2 }} ∪ {{ ext }} // env.
+Add Parametric Morphism {av} ext : (@PacketAsCollectionOfVariables av)
+    with signature (eq ==> eq ==> eq ==> eq ==> eq ==> eq ==> (TelEq ext) ==> eq ==> (TelEq ext))
+      as PacketAsCollectionOfVariables_TelEq_morphism.
 Proof.
-  intros.
-  setoid_rewrite Propagate_anonymous_ret.
-  hoare.
-  move_to_front vret2.
-  move_to_front vret1.
-  change init1 with (fst init).
-  change init2 with (snd init).
-  eapply @CompileLoopBase2; eassumption.
+  unfold PacketAsCollectionOfVariables; intros * teq **.
+  repeat (apply TelEq_chomp_head; red; intros).
+  assumption.
 Qed.
 
-Lemma CompileCompose_init :
-  forall {av} E B (transformer: Transformer.Transformer B) enc1 enc2
-    (vstream: NameTag av B) (vcache: NameTag av E) (cache: E)
-    tenv tenv' tenv'' ext env p1 p2,
-    {{ [[ vstream  <--  Transformer.transform_id as _ ]]
-         :: [[ vcache  <--  cache as _ ]]
-         :: tenv }}
-      p1
-    {{ [[ NTNone  <--  enc1 cache as encoded1 ]]
-         :: [[ vstream  <--  Transformer.transform Transformer.transform_id (fst encoded1) as stream1 ]]
-         :: [[ vcache  <--  (snd encoded1) as cache1 ]]
-         :: tenv' }} ∪ {{ ext }} // env ->
-    (let encoded1 := enc1 cache in
-     {{ [[ vstream  <--  (fst encoded1) as stream1 ]]
-         :: [[ vcache  <--  (snd encoded1) as cache1 ]]
-          :: tenv' }}
-       p2
-     {{ [[ NTNone  <--  enc2 (snd encoded1) as encoded2 ]]
-          :: [[ vstream  <--  Transformer.transform (fst encoded1) (fst encoded2) as stream2 ]]
-          :: [[ vcache  <--  (snd encoded2) as cache2 ]]
-          :: tenv'' }} ∪ {{ ext }} // env) ->
-    {{ [[ vstream  <--  Transformer.transform_id as _ ]]
-         :: [[ vcache  <--  cache as _ ]]
-         :: tenv }}
-      (Seq p1 p2)
-    {{ [[ NTNone  <--  @Compose.compose E B transformer enc1 enc2 cache as composed ]]
-         :: [[ vstream  <--  (fst composed) as stream ]]
-         :: [[ vcache  <--  (snd composed) as cache ]]
-         :: tenv'' }} ∪ {{ ext }} // env.
+Add Parametric Morphism {av} ext : (@DnsCacheAsCollectionOfVariables av)
+    with signature (eq ==> eq ==> eq ==> (TelEq ext) ==> eq ==> (TelEq ext))
+      as DnsCacheAsCollectionOfVariables_TelEq_morphism.
 Proof.
-  intros.
-  setoid_rewrite <- (Transformer.transform_id_left (fst _)).
-  eapply CompileCompose_spec'; cbv zeta.
-  eassumption.
-  setoid_rewrite Transformer.transform_id_left; eassumption.
-Qed.
-
-Lemma ProgOk_Transitivity_DropName :
-  forall {av A} {W: FacadeWrapper (Value av) A} env ext (t1: Telescope av) t2 prog1 prog2 (k: string) (v: Comp A),
-    {{ t1 }}                     prog1      {{ [[`k <~~ v as _]]::DropName k t1 }}     ∪ {{ ext }} // env ->
-    {{ [[`k <~~ v as _]]::DropName k t1 }}      prog2      {{ [[`k <~~ v as kk]]::t2 kk }} ∪ {{ ext }} // env ->
-    {{ t1 }}                Seq prog1 prog2 {{ [[`k <~~ v as kk]]::t2 kk }} ∪ {{ ext }} // env.
-Proof.
-  eauto using CompileSeq.
+  unfold DnsCacheAsCollectionOfVariables; intros * teq **.
+  repeat (apply TelEq_chomp_head; red; intros).
+  assumption.
 Qed.
 
 Lemma ProgOk_Transitivity_First :
@@ -734,35 +296,6 @@ Lemma ProgOk_Transitivity_First :
     {{ [[k <~~ v1 as _]]::t1 }}  Seq prog1 prog2 {{ [[k <~~ v2 as kk]]::t2 kk }} ∪ {{ ext }} // env.
 Proof.
   eauto using CompileSeq.
-Qed.
-
-Lemma IList_encode_bools_is_copy:
-  forall bits cache,
-    (IList.IList_encode' DnsMap.cache Core.btransformer Bool.Bool_encode bits cache) =
-    (bits, {| DnsMap.eMap := DnsMap.eMap cache;
-              DnsMap.dMap := DnsMap.dMap cache;
-              DnsMap.offs := DnsMap.offs cache + (N.of_nat (List.length bits)) |}).
-Proof.
-  Opaque N.of_nat.
-  induction bits; destruct cache; simpl in *.
-  + rewrite N.add_0_r; reflexivity.
-  + rewrite IHbits; simpl.
-    rewrite <- N.add_assoc, N.add_1_l, Nat2N.inj_succ; reflexivity.
-    Transparent N.of_nat.
-Qed.
-
-Definition EncodeAndPad n length :=
-  let encoded := FixInt.encode' n in
-  FixInt.pad encoded (length - Datatypes.length encoded).
-
-Lemma FixInt_encode_is_copy {size}:
-  forall num cache,
-    (FixInt.FixInt_encode (size := size) num cache) =
-    (EncodeAndPad (`num) size, {| DnsMap.eMap := DnsMap.eMap cache;
-                                  DnsMap.dMap := DnsMap.dMap cache;
-                                  DnsMap.offs := DnsMap.offs cache + (N.of_nat size) |}).
-Proof.
-  destruct cache; reflexivity.
 Qed.
 
 Lemma CompileCallWrite16:
@@ -783,12 +316,6 @@ Proof.
   hoare.
   hoare.
   hoare.
-Admitted.
-
-Definition List16AsWord (ls: {s : list bool | Datatypes.length s = 16}) : W.
-Admitted.
-
-Lemma EncodeAndPad_ListAsWord : forall ls, `ls = EncodeAndPad (Word.wordToN (List16AsWord ls)) 16.
 Admitted.
 
 Ltac _compile_callWrite16 :=
@@ -828,7 +355,7 @@ Ltac keep_unmodified_packet :=
   instantiate_tail_of_post find_packet.
 
 Ltac compile_compose :=
-  (eapply CompileCompose_spec' || eapply CompileCompose_init); intros.
+  (eapply CompileCompose || eapply CompileCompose_init); intros.
 
 Ltac packet_start_compiling :=
   repeat match goal with
@@ -909,16 +436,6 @@ Proof.
   hoare; hoare.
 Admitted.
 
-Ltac _packet_encode_FixInt :=
-  match_ProgOk
-    ltac:(fun prog pre post ext env =>
-            match constr:post with
-            | [[ret (FixInt.FixInt_encode _ _) as _]] :: _ =>
-              rewrite FixInt_encode_is_copy;
-              setoid_rewrite Propagate_anonymous_ret; simpl;
-              apply ProgOk_Transitivity_First
-            end).
-
 Lemma CompileCallListResourceLength:
   forall (vlst varg : string) (tenv : Telescope ADTValue) (ext : StringMap.t (Value ADTValue))
     env (lst : list resource_t)
@@ -941,6 +458,16 @@ Lemma CompileCallListQuestionLength:
 Proof.
 Admitted.
 
+Ltac _packet_encode_FixInt :=
+  match_ProgOk
+    ltac:(fun prog pre post ext env =>
+            match constr:post with
+            | [[ret (FixInt.FixInt_encode _ _) as _]] :: _ =>
+              rewrite FixInt_encode_is_copy;
+              setoid_rewrite Propagate_anonymous_ret; simpl;
+              apply ProgOk_Transitivity_First
+            end).
+
 Ltac _compile_CallListLength :=
   match_ProgOk
     ltac:(fun _ _ post _ _ =>
@@ -955,7 +482,8 @@ Ltac _compile_CallListLength :=
                         | context[Cons (NTSome ?k) (ret lst) _] =>
                           (eapply (CompileCallListResourceLength k) ||
                            eapply (CompileCallListQuestionLength k));
-                          [ decide_TelEq_instantiate ]
+                          [ unfold DnsCacheAsCollectionOfVariables; (* FIXME autounfold *)
+                            decide_TelEq_instantiate ]
                         end)
             end).
 
@@ -967,41 +495,6 @@ Ltac _compile_CallAllocString :=
               let vtmp := gensym "tmp" in
               eapply (CompileCallAllocString vtmp)
             end).
-
-Lemma NToWord_of_nat:
-  forall (sz : nat) (n : nat),
-    Word.NToWord (N.of_nat n) = Word.natToWord sz n.
-Proof.
-  intros; rewrite Word.NToWord_nat, Nat2N.id; reflexivity.
-Qed.
-
-Lemma NToWord_WordToN:
-  forall (sz : nat) (w : Word.word sz),
-    Word.NToWord (Word.wordToN w) = w.
-Proof.
-  intros; rewrite Word.NToWord_nat, Word.wordToN_nat, Nat2N.id.
-  apply Word.natToWord_wordToNat.
-Qed.
-
-Lemma length_of_fixed_length_list :
-  forall {size} (ls: {s : list bool | Datatypes.length s = size}),
-    List.length (`ls) = size.
-Proof.
-  destruct ls; auto.
-Qed.
-
-Lemma FixList_is_IList :
-  forall (A bin : Type) (cache : Cache.Cache) (transformer : Transformer.Transformer bin)
-    (A_encode : A -> Cache.CacheEncode -> bin * Cache.CacheEncode)
-    (xs : list A) (env : Cache.CacheEncode),
-    @FixList.FixList_encode' A bin cache transformer A_encode xs env =
-    @IList.IList_encode' A bin cache transformer A_encode xs env.
-Proof.
-  induction xs; simpl; intros.
-  + reflexivity.
-  + destruct (A_encode _ _).
-    rewrite IHxs; reflexivity.
-Qed.
 
 Create HintDb packet_autorewrite_db.
 Hint Rewrite -> @NToWord_of_nat : packet_autorewrite_db.
@@ -1034,22 +527,6 @@ Ltac _compile_rewrite_bind ::= fail.
 (*  Disable automatic decompilation for this file (it only orks for simple examples with no evars in the post) *)
 Ltac _compile_destructor ::= fail.
 
-Ltac compile_simple_inplace ::=
-  match_ProgOk                (* FIXME merge this upstream (made it faster in the failing case) *)
-  ltac:(fun prog pre post ext env =>
-          match post with
-          | Cons (NTSome ?s) (ret (?op ?a' ?b)) ?tenv' =>
-            match pre with
-            | context[Cons (NTSome ?s) (ret ?a) _] =>
-              unify a a';
-              is_word (op a b);
-              let facade_op := translate_op op in
-              move_to_front s;
-              first [ apply (CompileBinopOrTest_right_inPlace_tel facade_op)
-                    | apply (CompileBinopOrTest_right_inPlace_tel_generalized facade_op) ]
-            end
-          end).
-
 Ltac _packet_encode_step :=
   match goal with
   | _ => _packet_encode_cleanup
@@ -1063,159 +540,7 @@ Ltac _packet_encode_step :=
 Ltac _packet_encode_t :=
   repeat _packet_encode_step.
 
-
-Lemma CompileCompose_spec'' :
-  forall {av} E B (transformer: Transformer.Transformer B) enc1 enc2
-    (stream: B) (cache: E) (tenv tenv' tenv'': B -> E -> Telescope av) ext env p1 p2,
-    {{ tenv stream cache }}
-      p1
-    {{ [[ NTNone  <--  enc1 cache as encoded1 ]]
-         :: tenv' (Transformer.transform stream (fst encoded1)) (snd encoded1) }}
-    ∪ {{ ext }} // env ->
-    (let encoded1 := enc1 cache in
-     let stream1 := Transformer.transform stream (fst encoded1) in
-     {{ tenv' stream1 (snd encoded1) }}
-       p2
-     {{ [[ NTNone  <--  enc2 (snd encoded1) as encoded2 ]]
-          :: tenv'' (Transformer.transform stream1 (fst encoded2)) (snd encoded2) }}
-     ∪ {{ ext }} // env) ->
-    {{ tenv stream cache }}
-      (Seq p1 p2)
-    {{ [[ NTNone  <--  @Compose.compose E B transformer enc1 enc2 cache as composed ]]
-         :: tenv'' (Transformer.transform stream (fst composed)) (snd composed) }}
-    ∪ {{ ext }} // env.
-Proof.
-  repeat hoare.
-  setoid_rewrite Compose_compose_acc.
-  unfold compose_acc, encode_continue.
-  cbv zeta in *.
-  repeat rewrite @Propagate_anonymous_ret in *.
-  destruct (enc1 _); simpl in *; destruct (enc2 _); simpl in *;
-    rewrite Transformer.transform_assoc; assumption.
-Qed.
-
-Lemma CompileCompose_spec''' :
-  forall {av} E B (transformer: Transformer.Transformer B) enc1 enc2
-    (vstream: NameTag av B) (stream: B) (cache: E)
-    cacheF (tenv tenv' tenv'': Telescope av) ext env p1 p2,
-    {{ [[ vstream  <--  stream as _ ]]
-         :: cacheF tenv cache }}
-      p1
-    {{ [[ NTNone  <--  enc1 cache as encoded1 ]]
-         :: [[ vstream  <--  Transformer.transform stream (fst encoded1) as stream1 ]]
-         :: cacheF tenv' (snd encoded1) }} ∪ {{ ext }} // env ->
-    (let encoded1 := enc1 cache in
-     let stream1 := Transformer.transform stream (fst encoded1) in
-     {{ [[ vstream  <--  stream1 as _ ]]
-          :: cacheF tenv' (snd encoded1) }}
-       p2
-     {{ [[ NTNone  <--  enc2 (snd encoded1) as encoded2 ]]
-          :: [[ vstream  <--  Transformer.transform stream1 (fst encoded2) as stream2 ]]
-          :: cacheF tenv'' (snd encoded2) }} ∪ {{ ext }} // env) ->
-    {{ [[ vstream  <--  stream as _ ]]
-         :: cacheF tenv cache }}
-      (Seq p1 p2)
-    {{ [[ NTNone  <--  @Compose.compose E B transformer enc1 enc2 cache as composed ]]
-         :: [[ vstream  <--  Transformer.transform stream (fst composed) as stream ]]
-         :: cacheF tenv'' (snd composed) }} ∪ {{ ext }} // env.
-Proof.
-  repeat hoare.
-  setoid_rewrite Compose_compose_acc.
-  unfold compose_acc, encode_continue.
-  cbv zeta in H0.
-  repeat setoid_rewrite Propagate_anonymous_ret.
-  repeat setoid_rewrite Propagate_anonymous_ret in H.
-  repeat setoid_rewrite Propagate_anonymous_ret in H0.
-  destruct (enc1 _); simpl in *.
-  destruct (enc2 _); simpl in *.
-  rewrite Transformer.transform_assoc; assumption.
-Qed.
-
-(* Lemma CompileCompose_init' : *)
-(*   forall {av} E B (transformer: Transformer.Transformer B) enc1 enc2 *)
-(*     (cache: E) (tenv tenv' tenv'': B -> E -> Telescope av) ext env p1 p2, *)
-(*     {{ tenv Transformer.transform_id cache }} *)
-(*       p1 *)
-(*     {{ [[ NTNone  <--  enc1 cache as encoded1 ]] *)
-(*          :: tenv' (Transformer.transform Transformer.transform_id (fst encoded1)) (snd encoded1) }} *)
-(*     ∪ {{ ext }} // env -> *)
-(*     (let encoded1 := enc1 cache in *)
-(*      {{ tenv' (fst encoded1) (snd encoded1) }} *)
-(*        p2 *)
-(*      {{ [[ NTNone  <--  enc2 (snd encoded1) as encoded2 ]] *)
-(*           :: tenv'' (Transformer.transform (fst encoded1) (fst encoded2)) (snd encoded2) }} *)
-(*      ∪ {{ ext }} // env) -> *)
-(*     {{ tenv Transformer.transform_id cache }} *)
-(*       (Seq p1 p2) *)
-(*     {{ [[ NTNone  <--  @Compose.compose E B transformer enc1 enc2 cache as composed ]] *)
-(*          :: tenv'' (fst composed) (snd composed) }} ∪ {{ ext }} // env. *)
-(* Proof. *)
-(*   intros. *)
-(*   setoid_rewrite <- (Transformer.transform_id_left (fst _)). *)
-(*   eapply CompileCompose_spec''; cbv zeta. *)
-(*   eassumption. *)
-(*   setoid_rewrite Transformer.transform_id_left; eassumption. *)
-(* Qed. *)
-
-Lemma CompileCompose_init'' :
-  forall {av} E B (transformer: Transformer.Transformer B) enc1 enc2
-    (cache: E) (tenv tenv' tenv'': B -> E -> Telescope av) ext env p1 p2,
-    {{ tenv Transformer.transform_id cache }}
-      p1
-    {{ [[ NTNone  <--  enc1 cache as encoded1 ]]
-         :: tenv' (Transformer.transform Transformer.transform_id (fst encoded1)) (snd encoded1) }}
-    ∪ {{ ext }} // env ->
-    (let encoded1 := enc1 cache in
-     {{ tenv' (fst encoded1) (snd encoded1) }}
-       p2
-     {{ [[ NTNone  <--  enc2 (snd encoded1) as encoded2 ]]
-          :: tenv'' (Transformer.transform (fst encoded1) (fst encoded2)) (snd encoded2) }}
-     ∪ {{ ext }} // env) ->
-    {{ tenv Transformer.transform_id cache }}
-      (Seq p1 p2)
-    {{ [[ NTNone  <--  @Compose.compose E B transformer enc1 enc2 cache as composed ]]
-         :: tenv'' (fst composed) (snd composed) }} ∪ {{ ext }} // env.
-Proof.
-  intros.
-  setoid_rewrite <- (Transformer.transform_id_left (fst _)).
-  eapply CompileCompose_spec''; cbv zeta.
-  eassumption.
-  setoid_rewrite Transformer.transform_id_left; eassumption.
-Qed.
-
-Lemma CompileCompose_init''' :
-  forall {av} E B (transformer: Transformer.Transformer B) enc1 enc2
-    (vstream: NameTag av B) (cache: E)
-    cacheF (tenv tenv' tenv'': Telescope av) ext env p1 p2,
-    {{ [[ vstream  <--  Transformer.transform_id as _ ]]
-         :: cacheF tenv cache }}
-      p1
-    {{ [[ NTNone  <--  enc1 cache as encoded1 ]]
-         :: [[ vstream  <--  Transformer.transform Transformer.transform_id (fst encoded1) as stream1 ]]
-         :: cacheF tenv' (snd encoded1) }} ∪ {{ ext }} // env ->
-    (let encoded1 := enc1 cache in
-     {{ [[ vstream  <--  (fst encoded1) as _ ]]
-          :: cacheF tenv' (snd encoded1) }}
-       p2
-     {{ [[ NTNone  <--  enc2 (snd encoded1) as encoded2 ]]
-          :: [[ vstream  <--  Transformer.transform (fst encoded1) (fst encoded2) as stream2 ]]
-          :: cacheF tenv'' (snd encoded2) }} ∪ {{ ext }} // env) ->
-    {{ [[ vstream  <--  Transformer.transform_id as _ ]]
-         :: cacheF tenv cache }}
-      (Seq p1 p2)
-    {{ [[ NTNone  <--  @Compose.compose E B transformer enc1 enc2 cache as composed ]]
-         :: [[ vstream  <--  (fst composed) as stream ]]
-         :: cacheF tenv'' (snd composed) }} ∪ {{ ext }} // env.
-Proof.
-  intros.
-  setoid_rewrite <- (Transformer.transform_id_left (fst _)).
-  eapply CompileCompose_spec'''; cbv zeta.
-  eassumption.
-  setoid_rewrite Transformer.transform_id_left; eassumption.
-Qed.
-
-
-Lemma CompileLoopBase2' :
+Lemma CompileLoopBase2 :
   forall {A1 A2 C}
     `{FacadeWrapper (Value QsADTs.ADTValue) A1}
     `{FacadeWrapper (Value QsADTs.ADTValue) C}
@@ -1253,15 +578,6 @@ Proof.
   generalize dependent init;
   induction lst; loop_t.
 
-Ltac decide_NotInTelescope ::=
-  progress repeat match goal with
-                  | _ => cleanup
-                  | _ => congruence
-                  | [  |- NotInTelescope _ Nil ] => reflexivity
-                  | [  |- NotInTelescope ?k (Cons _ _ _) ] => simpl
-                  | _ => auto 1  (* Added for tricky cases like CompileLoopBase2 *)
-                  end.
-
   move_to_front vtest;
     apply CompileWhileFalse_Loop; loop_t.
 
@@ -1296,43 +612,154 @@ Ltac decide_NotInTelescope ::=
   loop_t.
 Qed.
 
-Lemma CompileLoop2_destructed' :
+
+Lemma CompileLoop2_destructed :
   forall {A1 A2 C}
     `{FacadeWrapper (Value QsADTs.ADTValue) A1}
     `{FacadeWrapper (Value QsADTs.ADTValue) C}
     `{FacadeWrapper (Value QsADTs.ADTValue) (list C)}
     vhead vtest vlst vret1
     (lst: list C) init1 init2 (init := (init1, init2))
-    tenvF (f: A1 * A2 -> C -> A1 * A2) tenv tenv'
+    tenvF (f: A1 * A2 -> C -> A1 * A2) tenv0 tenv tenv'
     env (ext: StringMap.t (Value QsADTs.ADTValue))
     fpop fempty fdealloc facadeBody facadeConclude,
     (* GLabelMap.MapsTo fpop (Axiomatic (QsADTs.TupleList_pop)) env -> *)
     (* GLabelMap.MapsTo fempty (Axiomatic (QsADTs.TupleList_empty)) env -> *)
     (* GLabelMap.MapsTo fdealloc (Axiomatic (QsADTs.TupleList_delete)) env -> *)
     PreconditionSet tenv ext [[[vhead; vtest; vlst; vret1]]] ->
+    TelEq ext tenv0 ([[`vlst <-- lst as _]] :: [[`vret1 <-- init1 as _]] :: tenvF tenv init2) ->
     (forall v, NotInTelescope vtest (tenvF tenv v)) ->
     {{ [[`vret1 <-- fst (fold_left f lst init) as _]] :: tenvF tenv (snd (fold_left f lst init)) }}
       facadeConclude
-    {{ [[`vret1 <-- fst (fold_left f lst init) as v1]] :: tenvF tenv' (snd (fold_left f lst init)) }}
-    ∪ {{ ext }} // env ->
+      {{ [[`vret1 <-- fst (fold_left f lst init) as v1]] :: tenvF tenv' (snd (fold_left f lst init)) }}
+      ∪ {{ ext }} // env ->
     (forall head (acc1: A1) (acc2: A2) (s: list C),
         {{ [[`vhead <-- head as _]] :: [[`vret1 <-- acc1 as _]] :: tenvF tenv acc2 }}
           facadeBody
-        {{ [[`vret1 <-- fst (f (acc1, acc2) head) as _]] :: tenvF tenv (snd (f (acc1, acc2) head)) }} ∪
-        {{ [vtest <-- wrap (bool2w false)] :: [vlst <-- wrap s] :: ext }} // env) ->
-    {{ [[`vlst <-- lst as _]] :: [[`vret1 <-- init1 as _]] :: tenvF tenv init2 }}
+          {{ [[`vret1 <-- fst (f (acc1, acc2) head) as _]] :: tenvF tenv (snd (f (acc1, acc2) head)) }} ∪
+          {{ [vtest <-- wrap (bool2w false)] :: [vlst <-- wrap s] :: ext }} // env) ->
+    {{ tenv0 }}
       (Seq (Seq (Fold vhead vtest vlst fpop fempty facadeBody) (Call (DummyArgument vtest) fdealloc (vlst :: nil))) facadeConclude)
-    {{ [[ ret (fold_left f lst init) as folded ]]
-         :: [[`vret1 <-- fst folded as v1]]
-         :: tenvF tenv' (snd folded) }} ∪ {{ ext }} // env.
+      {{ [[ ret (fold_left f lst init) as folded ]]
+           :: [[`vret1 <-- fst folded as v1]]
+           :: tenvF tenv' (snd folded) }} ∪ {{ ext }} // env.
 Proof.
   intros.
+  rewrite H3.
   setoid_rewrite Propagate_anonymous_ret.
   hoare.
   change init1 with (fst init).
   change init2 with (snd init).
-  eapply @CompileLoopBase2'; eassumption.
+  eapply @CompileLoopBase2; eassumption.
 Qed.
+
+Inductive EvarTag {T A} (a: A) (t: T) := __EvarTag.
+
+Ltac _packet_encode__clear_EvarTags :=
+  repeat match goal with
+         | [ H: EvarTag ?v ?tag |- _ ] => try unify v tag; clear H
+         end.
+
+Ltac specialize_function_with_evar f tag :=
+  lazymatch type of f with
+  | ?A -> _ => let a := fresh in
+             let old_f := fresh "old" in
+             evar (a: A);
+             rename f into old_f;
+             pose (old_f a) as f;
+             lazymatch constr:tag with
+             | Some ?t => pose proof (__EvarTag a t)
+             | _ => idtac
+             end;
+             unfold old_f, a in *;
+             clear old_f; clear a
+  end.
+
+Ltac specialize_function_with_evars f :=
+  repeat (specialize_function_with_evar f None).
+
+Ltac create_packet_evar name :=
+  pose @Build_packet_t as name;
+  specialize_function_with_evars name.
+
+Ltac _packet_encode_IList__rewrite_as_fold :=
+  lazymatch goal with         (* FIXME make this an autorewrite *)
+  | [  |- appcontext[IList.IList_encode' ?cache] ] =>
+    rewrite IList.IList_encode'_as_foldl;
+    rewrite (IList_post_transform_TelEq cache)
+  end.
+
+Ltac specialize_body hyp term :=
+  let new := fresh in
+  pose (hyp term) as fresh;
+  unfold hyp in *;
+  clear hyp;
+  rename fresh into hyp.
+
+Ltac _packet__havoc_packet_in_postcondition :=
+  let p := find_packet in
+  let p' := fresh in
+  lazymatch constr:p with
+  | @PacketAsCollectionOfVariables ?av ?x0 ?x1 ?x2 ?x3 ?x4 ?x5 ?tail ?p =>
+    let tail' := fresh in
+    create_packet_evar p';
+    pose (@PacketAsCollectionOfVariables av) as tail';
+    (* FIXME generalize this *)
+    specialize_function_with_evar tail' (Some x0);
+    specialize_function_with_evar tail' (Some x1);
+    specialize_function_with_evar tail' (Some x2);
+    specialize_function_with_evar tail' (Some x3);
+    specialize_function_with_evar tail' (Some x4);
+    specialize_function_with_evar tail' (Some x5);
+    specialize_body tail' tail;
+    specialize_body tail' p';
+    instantiate_tail_of_post tail';
+    unfold p', tail' in *; clear p'; clear tail'
+  end.
+
+Ltac delete_tagged_var_from_post var :=
+  (* Delete VAR from post-condition.
+     Since VAR doesn't appear litteraly in the post-condition, use an EvarTag
+     to find which evar to remove in the post instead. *)
+  lazymatch goal with
+  | [ H: EvarTag ?k (@NTSome ?av ?T var ?wrp) |- _ ] =>
+    let kk := fresh in
+    set (kk := k); (* Otherwise the match below fails *)
+    lazymatch goal with
+    | [  |- context[Cons (@NTSome av T var wrp) (ret ?old_val) _] ] =>
+      lazymatch goal with
+      | [  |- context[Cons kk ?new_val ?tenv] ] =>
+        unify k (@NTNone av T); unfold kk; clear kk;
+        unify (ret old_val) new_val;
+        setoid_rewrite (@Propagate_anonymous_ret _ _ tenv _ old_val)
+      end
+    end
+  end.
+
+Ltac _compile_Loop2 vlst :=
+  let vhead := gensym "head" in
+  let vtest := gensym "test" in
+  eapply (CompileLoop2_destructed vhead vtest vlst);
+  [ | unfold DnsCacheAsCollectionOfVariables; simpl; decide_TelEq_instantiate | idtac.. ].
+
+Ltac _packet_encode_IList__compile_loop :=
+  unfold PacketAsCollectionOfVariables; simpl;
+  match_ProgOk
+    ltac:(fun prog pre post ext env =>
+            match constr:post with
+            | appcontext[fold_left (IList.IList_encode'_body _ _ _) ?lst] =>
+              match constr:pre with
+              | context[Cons (NTSome ?vlst) (ret lst) _] =>
+                delete_tagged_var_from_post vlst;
+                _packet_encode__clear_EvarTags;
+                _compile_Loop2 vlst
+              end
+            end).
+
+Ltac _packet_encode_IList_compile :=
+  _packet_encode_IList__rewrite_as_fold;
+  _packet__havoc_packet_in_postcondition;
+  _packet_encode_IList__compile_loop.
 
 Example encode :
   ParametricExtraction
@@ -1347,14 +774,9 @@ Proof.
   start_compiling.
   packet_start_compiling.
 
-  (* FIXME use multiple variables for the cache *)
   eapply (ProgOk_Add_snd_ret (DnsCacheAsCollectionOfVariables (NTSome "eMap") (NTSome "dMap") (NTSome "offs"))).
 
   eapply CompileSeq; [ | repeat compile_compose]; _packet_encode_t.
-
-  Focus 2.
-  repeat ((eapply CompileCompose_spec''' || eapply CompileCompose_init'''); intros); _packet_encode_t.
-  Unfocus.
 
   Focus.
   _packet_encode_t.
@@ -1383,24 +805,6 @@ Proof.
   Unfocused.
 
   Focus.
-Ltac _compile_CallListLength ::=
-  match_ProgOk
-    ltac:(fun _ _ post _ _ =>
-            match constr:post with
-            | [[ _ <-- Word.natToWord 32 (Datatypes.length ?lst) as _]] :: _ =>
-              (* FIXME this should be an equivalent of find_in_ext *)
-              (* FIXME this shoud be more principled *)
-              unfold PacketAsCollectionOfVariables; simpl;
-              match_ProgOk
-                ltac:(fun _ pre _ _ _ =>
-                        match constr:pre with
-                        | context[Cons (NTSome ?k) (ret lst) _] =>
-                          (eapply (CompileCallListResourceLength k) ||
-                           eapply (CompileCallListQuestionLength k));
-                          [ unfold DnsCacheAsCollectionOfVariables; (* FIXME autounfold *)
-                            decide_TelEq_instantiate ]
-                        end)
-            end).
   _packet_encode_t.
   keep_unmodified_packet.
   instantiate (1 := Call (DummyArgument "tmp") ("admitted", "Increment counter in cache") nil); admit.
@@ -1424,253 +828,24 @@ Ltac _compile_CallListLength ::=
   instantiate (1 := Call (DummyArgument "tmp") ("admitted", "Increment cache counter") nil); admit.
   Unfocused.
 
-  Lemma IList_post_transform_TelEq :
-    forall {av} {A bin : Type}
-      (cache : Cache.Cache) (transformer : Transformer.Transformer bin)
-      (A_encode : A -> Cache.CacheEncode -> bin * Cache.CacheEncode)
-      (xs : list A) (base : bin) (env : Cache.CacheEncode)
-      k__stream (cacheF: Telescope av -> Cache.CacheEncode -> Telescope av) (tenv: Telescope av) ext,
-      let fold_on b :=
-          fold_left (IList.IList_encode'_body cache transformer A_encode) xs (b, env) in
-      TelEq ext
-        ([[ret (fold_on Transformer.transform_id) as folded]]
-           ::[[ k__stream <-- Transformer.transform base (fst folded) as _]] :: cacheF tenv (snd folded))
-        ([[ret (fold_on base) as folded]]
-           ::[[ k__stream <-- fst folded as _]] :: cacheF tenv (snd folded)).
-  Proof.
-    cbv zeta; intros.
-    setoid_rewrite Propagate_anonymous_ret.
-    rewrite (IList.IList_encode'_body_characterization _ _ _ _ base).
-    destruct (fold_left _ _ _); simpl; reflexivity.
-  Qed.
-
-  Inductive EvarTag {T A} (a: A) (t: T) := __EvarTag.
-
-  Ltac specialize_function_with_evar f tag :=
-    lazymatch type of f with
-    | ?A -> _ => let a := fresh in
-               let old_f := fresh "old" in
-               evar (a: A);
-               rename f into old_f;
-               pose (old_f a) as f;
-               lazymatch constr:tag with
-               | Some ?t => pose proof (__EvarTag a t)
-               | _ => idtac
-               end;
-               unfold old_f, a in *;
-               clear old_f; clear a
-    end.
-
-  Ltac specialize_function_with_evars f :=
-    repeat (specialize_function_with_evar f None).
-
-  Ltac create_packet_evar name :=
-    pose @Build_packet_t as name;
-    specialize_function_with_evars name.
-
-  Ltac _packet_encode_IList__rewrite_as_fold :=
-    lazymatch goal with         (* FIXME make this an autorewrite *)
-    | [  |- appcontext[IList.IList_encode' ?cache] ] =>
-      rewrite IList.IList_encode'_as_foldl;
-      rewrite (IList_post_transform_TelEq cache)
-    end.
-
-  Ltac specialize_body hyp term :=
-    let new := fresh in
-    pose (hyp term) as fresh;
-    unfold hyp in *;
-    clear hyp;
-    rename fresh into hyp.
-
-  Ltac _packet__havoc_packet_in_postcondition :=
-    let p := find_packet in
-    let p' := fresh in
-    lazymatch constr:p with
-    | @PacketAsCollectionOfVariables ?av ?x0 ?x1 ?x2 ?x3 ?x4 ?x5 ?tail ?p =>
-      let tail' := fresh in
-      create_packet_evar p';
-      pose (@PacketAsCollectionOfVariables av) as tail';
-      (* FIXME generalize this *)
-      specialize_function_with_evar tail' (Some x0);
-      specialize_function_with_evar tail' (Some x1);
-      specialize_function_with_evar tail' (Some x2);
-      specialize_function_with_evar tail' (Some x3);
-      specialize_function_with_evar tail' (Some x4);
-      specialize_function_with_evar tail' (Some x5);
-      specialize_body tail' tail;
-      specialize_body tail' p';
-      instantiate_tail_of_post tail';
-      unfold p', tail' in *; clear p'; clear tail'
-    end.
-
-  Ltac delete_tagged_var_from_post var :=
-    (* Delete VAR from post-condition.
-       Since VAR doesn't appear litteraly in the post-condition, use an EvarTag
-       to find which evar to remove in the post instead. *)
-    lazymatch goal with
-    | [ H: EvarTag ?k (@NTSome ?av ?T var ?wrp) |- _ ] =>
-      let kk := fresh in
-      set (kk := k); (* Otherwise the match below fails *)
-      lazymatch goal with
-      | [  |- context[Cons (@NTSome av T var wrp) (ret ?old_val) _] ] =>
-        lazymatch goal with
-        | [  |- context[Cons kk ?new_val ?tenv] ] =>
-          unify k (@NTNone av T); unfold kk; clear kk;
-          unify (ret old_val) new_val;
-          setoid_rewrite (@Propagate_anonymous_ret _ _ tenv _ old_val)
-        end
-      end
-    end.
-
-  Lemma CompileLoop2_destructed'' :
-    forall {A1 A2 C}
-      `{FacadeWrapper (Value QsADTs.ADTValue) A1}
-      `{FacadeWrapper (Value QsADTs.ADTValue) C}
-      `{FacadeWrapper (Value QsADTs.ADTValue) (list C)}
-      vhead vtest vlst vret1
-      (lst: list C) init1 init2 (init := (init1, init2))
-      tenvF (f: A1 * A2 -> C -> A1 * A2) tenv0 tenv tenv'
-      env (ext: StringMap.t (Value QsADTs.ADTValue))
-      fpop fempty fdealloc facadeBody facadeConclude,
-      (* GLabelMap.MapsTo fpop (Axiomatic (QsADTs.TupleList_pop)) env -> *)
-      (* GLabelMap.MapsTo fempty (Axiomatic (QsADTs.TupleList_empty)) env -> *)
-      (* GLabelMap.MapsTo fdealloc (Axiomatic (QsADTs.TupleList_delete)) env -> *)
-      PreconditionSet tenv ext [[[vhead; vtest; vlst; vret1]]] ->
-      TelEq ext tenv0 ([[`vlst <-- lst as _]] :: [[`vret1 <-- init1 as _]] :: tenvF tenv init2) ->
-      (forall v, NotInTelescope vtest (tenvF tenv v)) ->
-      {{ [[`vret1 <-- fst (fold_left f lst init) as _]] :: tenvF tenv (snd (fold_left f lst init)) }}
-        facadeConclude
-        {{ [[`vret1 <-- fst (fold_left f lst init) as v1]] :: tenvF tenv' (snd (fold_left f lst init)) }}
-        ∪ {{ ext }} // env ->
-      (forall head (acc1: A1) (acc2: A2) (s: list C),
-          {{ [[`vhead <-- head as _]] :: [[`vret1 <-- acc1 as _]] :: tenvF tenv acc2 }}
-            facadeBody
-            {{ [[`vret1 <-- fst (f (acc1, acc2) head) as _]] :: tenvF tenv (snd (f (acc1, acc2) head)) }} ∪
-            {{ [vtest <-- wrap (bool2w false)] :: [vlst <-- wrap s] :: ext }} // env) ->
-      {{ tenv0 }}
-        (Seq (Seq (Fold vhead vtest vlst fpop fempty facadeBody) (Call (DummyArgument vtest) fdealloc (vlst :: nil))) facadeConclude)
-        {{ [[ ret (fold_left f lst init) as folded ]]
-             :: [[`vret1 <-- fst folded as v1]]
-             :: tenvF tenv' (snd folded) }} ∪ {{ ext }} // env.
-  Proof.
-    intros.
-    rewrite H3.
-    setoid_rewrite Propagate_anonymous_ret.
-    hoare.
-    change init1 with (fst init).
-    change init2 with (snd init).
-    eapply @CompileLoopBase2'; eassumption.
-  Qed.
-
-  Ltac _packet_encode_IList__compile_loop :=
-    unfold PacketAsCollectionOfVariables; simpl;
-    match_ProgOk
-      ltac:(fun prog pre post ext env =>
-              match constr:post with
-              | appcontext[fold_left (IList.IList_encode'_body _ _ _) ?lst] =>
-                match constr:pre with
-                | context[Cons (NTSome ?vlst) (ret lst) _] =>
-                  delete_tagged_var_from_post vlst;
-                  let vhead := gensym "head" in
-                  let vtest := gensym "test" in
-                  eapply (CompileLoop2_destructed'' vhead vtest vlst);
-                  [ | unfold DnsCacheAsCollectionOfVariables; simpl; decide_TelEq_instantiate | idtac.. ]
-                end
-              end).
-
-  Ltac _packet_encode_IList_compile :=
-    _packet_encode_IList__rewrite_as_fold;
-    _packet__havoc_packet_in_postcondition;
-    _packet_encode_IList__compile_loop.
-
-  Add Parametric Morphism {av} ext : (@DnsCacheAsCollectionOfVariables av)
-    with signature (eq ==> eq ==> eq ==> (TelEq ext) ==> eq ==> (TelEq ext))
-      as DnsCacheAsCollectionOfVariables_TelEq_morphism.
-  Proof.
-    unfold DnsCacheAsCollectionOfVariables; intros * teq **.
-    repeat (apply TelEq_chomp_head; red; intros).
-    assumption.
-  Qed.
-
   Focus.
   _packet_encode_t.
   _packet_encode_IList_compile.
-  compile_do_side_conditions.
+  _packet_encode_t.
   _packet_encode_t.
   unfold DnsCacheAsCollectionOfVariables; decide_NotInTelescope.
   _packet_encode_t.
   instantiate (1 := Call (DummyArgument "tmp") ("admitted", "Encode question") nil); admit.
   Unfocused.
 
-  (* Lemma antiChomp: *)
-  (*   forall (av A : Type) (H : FacadeWrapper (Value av) A) *)
-  (*     (env : Env av) (key : StringMap.key) (v : A) *)
-  (*     (prog : Stmt) (tail1 tail2 : Telescope av) *)
-  (*     (ext : StringMap.t (Value av)), *)
-  (*     key ∉ ext -> *)
-  (*     {{ [[ `key  <--  v as kk]]::tail1 }} *)
-  (*       prog *)
-  (*     {{ [[ `key  <--  v as kk]]::tail2 }} ∪ {{ ext }} // env -> *)
-  (*     {{ tail1 }} *)
-  (*       prog *)
-  (*     {{ tail2 }} ∪ {{ [key <-- wrap v]::ext }} // env. *)
-  (* Proof. *)
-  (*   SameValues_Facade_t; *)
-  (*   change tail1 with ((fun v => tail1) v) in H2; *)
-  (*   apply Cons_PopExt in H2; *)
-  (*   SameValues_Facade_t. *)
-  (* Qed. *)
+  (* Note: One could also never unfold PacketAsCollectionOfVariables and
+     DnsCacheAsCollectionOfVariables (and instead find the variable to loop on
+     by copying the precondition into the context and unfolding locally. *)
 
   Focus.
   _packet_encode_t.
-  _packet_encode_IList__rewrite_as_fold.
-  _packet__havoc_packet_in_postcondition.
-
-  Ltac _packet_encode__clear_EvarTags :=
-    repeat match goal with
-           | [ H: EvarTag ?v ?tag |- _ ] => try unify v tag; clear H
-           end.
-
-  Ltac _compile_Loop2 vlst :=
-    let vhead := gensym "head" in
-    let vtest := gensym "test" in
-    eapply (CompileLoop2_destructed'' vhead vtest vlst);
-    [ | unfold DnsCacheAsCollectionOfVariables; simpl; decide_TelEq_instantiate | idtac.. ].
-
-  Ltac _packet_encode_IList__compile_loop ::=
-    unfold PacketAsCollectionOfVariables; simpl;
-    match_ProgOk
-      ltac:(fun prog pre post ext env =>
-              match constr:post with
-              | appcontext[fold_left (IList.IList_encode'_body _ _ _) ?lst] =>
-                match constr:pre with
-                | context[Cons (NTSome ?vlst) (ret lst) _] =>
-                  delete_tagged_var_from_post vlst;
-                  _packet_encode__clear_EvarTags;
-                  _compile_Loop2 vlst
-                end
-              end).
-
-  Ltac decide_TelEq_instantiate_step ::=
-    match goal with
-    | [  |- TelEq _ ?from ?to ] =>
-      match constr:((from, to)) with
-      | _ => rewrite DropName_Cons_Some_eq by congruence
-      | _ => rewrite DropName_Cons_Some_neq by congruence
-      | _ => (is_evar from || is_evar to); apply TelEq_refl
-      | (Cons NTNone _ _, _) => apply TelEq_chomp_None_left; [ eexists; reflexivity | red; intros ]
-      | (_, Cons NTNone _ _) => apply TelEq_chomp_None_right; [ eexists; reflexivity | red; intros ]
-      | (Cons ?k _ _, ?t) => decide_TelEq_instantiate_do_swaps k t; apply TelEq_chomp_head; red; intros
-      | (?t, Cons ?k _ _) => decide_TelEq_instantiate_do_swaps k t; apply TelEq_chomp_head; red; intros
-      | context [DropName ?k ?tenv] => first [ is_dirty_telescope tenv; fail 1 |
-                                              rewrite (DropName_NotInTelescope tenv k) by eauto ]
-      | _ => apply TelEq_refl
-      end
-    end.
-
-  _packet_encode_IList__compile_loop.
-  (* Note: One could also never unfold PacketAsCollectionOfVariables and DnsCacheAsCollectionOfVariables (and instead find the variable to loop on by copying the precondition into the context and unfolding locally. *)
-  compile_do_side_conditions.
+  _packet_encode_IList_compile.
+  _packet_encode_t.
   _packet_encode_t; unfold DnsCacheAsCollectionOfVariables; decide_NotInTelescope.
   _packet_encode_t.
   instantiate (1 := Call (DummyArgument "tmp") ("admitted", "Encode answer") nil); admit.
@@ -1679,7 +854,7 @@ Ltac _compile_CallListLength ::=
   Focus.
   _packet_encode_t.
   _packet_encode_IList_compile.
-  compile_do_side_conditions.
+  _packet_encode_t.
   _packet_encode_t; unfold DnsCacheAsCollectionOfVariables; decide_NotInTelescope.
   _packet_encode_t.
   instantiate (1 := Call (DummyArgument "tmp") ("admitted", "Encode authority") nil); admit.
@@ -1688,15 +863,14 @@ Ltac _compile_CallListLength ::=
   Focus.
   _packet_encode_t.
   _packet_encode_IList_compile.
-  compile_do_side_conditions.
+  _packet_encode_t.
   _packet_encode_t; unfold DnsCacheAsCollectionOfVariables; decide_NotInTelescope.
   _packet_encode_t.
   instantiate (1 := Call (DummyArgument "tmp") ("admitted", "Encode additional") nil); admit.
   Unfocused.
 
+  _packet_encode_t.
   repeat lazymatch goal with
-         | [  |- context[fst (?a, ?b)] ] => change (fst (a, b)) with a
-         | [  |- context[snd (?a, ?b)] ] => change (snd (a, b)) with b
          | [  |- context[Transformer.transform nil _] ] => setoid_rewrite @Transformer.transform_id_left
          | [  |- context[Transformer.transform _ nil] ] => setoid_rewrite @Transformer.transform_id_right
          end.
