src/CertifiedExtraction/Benchmarks/BinEncodersProperties.v
@@ -1,0 +1,123 @@
+Require Import BinEncoders.Env.Examples.Dns.
+Require Import Bedrock.Memory.
+Require Import NArith.
+
+Unset Implicit Arguments.
+
+Definition encode_continue {E B}
+           (transformer : Transformer.Transformer B)
+           (encode : E -> B * E)
+           acc :=
+  let (p, e') := encode (snd acc) in
+  (Transformer.transform (fst acc) p, e').
+
+Definition compose_acc {E B}
+           (transformer : Transformer.Transformer B)
+           (encode1 : E -> B * E)
+           (encode2 : E -> B * E) e0 :=
+  encode_continue transformer encode2 (encode1 e0).
+
+Lemma Compose_compose_acc {E B} :
+  forall transformer encode1 encode2 e0,
+    @Compose.compose E B transformer encode1 encode2 e0 =
+    @compose_acc E B transformer encode1 encode2 e0.
+Proof.
+  intros; unfold compose_acc, Compose.compose, encode_continue.
+  destruct (encode1 _); simpl; destruct (encode2 _); reflexivity.
+Qed.
+
+Lemma IList_encode_bools_is_copy:
+  forall bits cache,
+    (IList.IList_encode' DnsMap.cache Core.btransformer Bool.Bool_encode bits cache) =
+    (bits, {| DnsMap.eMap := DnsMap.eMap cache;
+              DnsMap.dMap := DnsMap.dMap cache;
+              DnsMap.offs := DnsMap.offs cache + (N.of_nat (List.length bits)) |}).
+Proof.
+  Opaque N.of_nat.
+  induction bits; destruct cache; simpl in *.
+  + rewrite N.add_0_r; reflexivity.
+  + rewrite IHbits; simpl.
+    rewrite <- N.add_assoc, N.add_1_l, Nat2N.inj_succ; reflexivity.
+    Transparent N.of_nat.
+Qed.
+
+Definition EncodeAndPad n length :=
+  let encoded := FixInt.encode' n in
+  FixInt.pad encoded (length - Datatypes.length encoded).
+
+Lemma FixInt_encode_is_copy {size}:
+  forall num cache,
+    (FixInt.FixInt_encode (size := size) num cache) =
+    (EncodeAndPad (proj1_sig num) size, {| DnsMap.eMap := DnsMap.eMap cache;
+                                           DnsMap.dMap := DnsMap.dMap cache;
+                                           DnsMap.offs := DnsMap.offs cache + (N.of_nat size) |}).
+Proof.
+  destruct cache; reflexivity.
+Qed.
+
+
+Definition List16AsWord (ls: {s : list bool | Datatypes.length s = 16}) : W.
+Admitted.
+
+Lemma EncodeAndPad_ListAsWord : forall ls, proj1_sig ls = EncodeAndPad (Word.wordToN (List16AsWord ls)) 16.
+Admitted.
+
+Lemma NToWord_of_nat:
+  forall (sz : nat) (n : nat),
+    Word.NToWord _ (N.of_nat n) = Word.natToWord sz n.
+Proof.
+  intros; rewrite Word.NToWord_nat, Nat2N.id; reflexivity.
+Qed.
+
+Lemma NToWord_WordToN:
+  forall (sz : nat) (w : Word.word sz),
+    Word.NToWord _ (Word.wordToN w) = w.
+Proof.
+  intros; rewrite Word.NToWord_nat, Word.wordToN_nat, Nat2N.id.
+  apply Word.natToWord_wordToNat.
+Qed.
+
+Lemma length_of_fixed_length_list :
+  forall {size} (ls: {s : list bool | Datatypes.length s = size}),
+    List.length (proj1_sig ls) = size.
+Proof.
+  destruct ls; auto.
+Qed.
+
+Lemma FixList_is_IList :
+  forall (A bin : Type) (cache : Cache.Cache) (transformer : Transformer.Transformer bin)
+    (A_encode : A -> Cache.CacheEncode -> bin * Cache.CacheEncode)
+    (xs : list A) (env : Cache.CacheEncode),
+    @FixList.FixList_encode' A bin cache transformer A_encode xs env =
+    @IList.IList_encode' A bin cache transformer A_encode xs env.
+Proof.
+  induction xs; simpl; intros.
+  + reflexivity.
+  + destruct (A_encode _ _).
+    rewrite IHxs; reflexivity.
+Qed.
+
+Require Import
+        CertifiedExtraction.Core
+        CertifiedExtraction.ExtendedLemmas
+        CertifiedExtraction.PropertiesOfTelescopes.
+
+Lemma IList_post_transform_TelEq :
+  forall {av} {A bin : Type}
+    (cache : Cache.Cache) (transformer : Transformer.Transformer bin)
+    (A_encode : A -> Cache.CacheEncode -> bin * Cache.CacheEncode)
+    (xs : list A) (base : bin) (env : Cache.CacheEncode)
+    k__stream (cacheF: Telescope av -> Cache.CacheEncode -> Telescope av) (tenv: Telescope av) ext,
+    let fold_on b :=
+        List.fold_left (IList.IList_encode'_body cache transformer A_encode) xs (b, env) in
+    TelEq ext
+      ([[ret (fold_on Transformer.transform_id) as folded]]
+         ::[[ k__stream <-- Transformer.transform base (fst folded) as _]] :: cacheF tenv (snd folded))
+      ([[ret (fold_on base) as folded]]
+         ::[[ k__stream <-- fst folded as _]] :: cacheF tenv (snd folded)).
+Proof.
+  cbv zeta; intros.
+  setoid_rewrite Propagate_anonymous_ret.
+  rewrite (IList.IList_encode'_body_characterization _ _ _ _ base).
+  destruct (List.fold_left _ _ _); simpl; reflexivity.
+Qed.
